Low level Merkle tree hash function parameterization

secure_api/merkle_tree/MerkleTree.New.High.Correct.Base.fst
@@ -76,7 +76,7 @@ let rec mt_hashes_lth_inv_empty #hsz lv =
   else mt_hashes_lth_inv_empty #hsz (lv + 1)
 
 val mt_hashes_next_rel:
-  #hsz:pos -> #f:MTS.tag_fun_t #hsz ->
+  #hsz:pos -> #f:MTS.hash_fun_t #hsz ->
   j:nat ->
   hs:hashes #hsz {S.length hs = j} ->
   nhs:hashes #hsz {S.length nhs = j / 2} ->
@@ -90,7 +90,7 @@ let mt_hashes_next_rel #hsz #f j hs nhs =
 #push-options "--max_fuel 2"
 
 val mt_hashes_inv:
-  #hsz:pos -> #f:MTS.tag_fun_t #hsz ->
+  #hsz:pos -> #f:MTS.hash_fun_t #hsz ->
   lv:nat{lv < 32} ->
   j:nat{j < pow2 (32 - lv)} ->
   fhs:hashess #hsz {S.length fhs = 32 /\ mt_hashes_lth_inv lv j fhs} ->
@@ -101,7 +101,7 @@ let rec mt_hashes_inv #hsz #f lv j fhs =
        mt_hashes_inv #_ #f (lv + 1) (j / 2) fhs)
 
 val mt_hashes_inv_empty:
-  #hsz:pos -> #f:MTS.tag_fun_t #hsz ->
+  #hsz:pos -> #f:MTS.hash_fun_t #hsz ->
   lv:nat{lv < 32} ->
   Lemma (requires True)
         (ensures (mt_hashes_lth_inv_empty #hsz lv;
@@ -113,7 +113,7 @@ let rec mt_hashes_inv_empty #hsz #f lv =
         mt_hashes_inv_empty #_ #f (lv + 1))
 
 val mt_hashes_lth_inv_equiv:
-  #hsz:pos -> #f:MTS.tag_fun_t #hsz ->
+  #hsz:pos -> #f:MTS.hash_fun_t #hsz ->
   lv:nat{lv < 32} ->
   j:nat{j < pow2 (32 - lv)} ->
   fhs1:hashess{S.length fhs1 = 32} ->
@@ -130,7 +130,7 @@ let rec mt_hashes_lth_inv_equiv #hsz #f lv j fhs1 fhs2 =
 #pop-options // --max_fuel = 2
 
 val mt_hashes_inv_equiv:
-  #hsz:pos -> #f:MTS.tag_fun_t #hsz ->
+  #hsz:pos -> #f:MTS.hash_fun_t #hsz ->
   lv:nat{lv < 32} ->
   j:nat{j < pow2 (32 - lv)} ->
   fhs1:hashess #hsz {S.length fhs1 = 32 /\ mt_hashes_lth_inv lv j fhs1} ->
@@ -146,7 +146,7 @@ let rec mt_hashes_inv_equiv #hsz #f lv j fhs1 fhs2 =
        mt_hashes_inv_equiv #_ #f (lv + 1) (j / 2) fhs1 fhs2)
 
 val merge_hs:
-  #hsz:pos -> #f:MTS.tag_fun_t #hsz ->
+  #hsz:pos -> #f:MTS.hash_fun_t #hsz ->
   hs1:hashess #hsz ->
   hs2:hashess #hsz {S.length hs1 = S.length hs2} ->
   GTot (mhs:hashess #hsz {S.length mhs = S.length hs1})
@@ -157,7 +157,7 @@ let rec merge_hs #hsz #f hs1 hs2 =
                (merge_hs #_ #f (S.tail hs1) (S.tail hs2)))
 
 val merge_hs_empty:
-  #hsz:pos -> #f:MTS.tag_fun_t #hsz ->
+  #hsz:pos -> #f:MTS.hash_fun_t #hsz ->
   len:nat ->
   Lemma (S.equal (merge_hs #_ #f (empty_hashes #hsz len) (empty_hashes #hsz len))
                  (empty_hashes #hsz len))
@@ -174,7 +174,7 @@ let rec merge_hs_empty #hsz #f len =
        merge_hs_empty #_ #f (len - 1))
 
 val merge_hs_index:
-  #hsz:pos -> #f:MTS.tag_fun_t #hsz ->
+  #hsz:pos -> #f:MTS.hash_fun_t #hsz ->
   hs1:hashess ->
   hs2:hashess{S.length hs1 = S.length hs2} ->
   i:nat{i < S.length hs1} ->
@@ -189,7 +189,7 @@ let rec merge_hs_index #hsz #f hs1 hs2 i =
   else merge_hs_index #_ #f (S.tail hs1) (S.tail hs2) (i - 1)
 
 val merge_hs_slice_equal:
-  #hsz:pos -> #f:MTS.tag_fun_t #hsz ->
+  #hsz:pos -> #f:MTS.hash_fun_t #hsz ->
   ahs1:hashess #hsz ->
   ahs2:hashess #hsz {S.length ahs1 = S.length ahs2} ->
   bhs1:hashess #hsz ->
@@ -207,7 +207,7 @@ let rec merge_hs_slice_equal #_ #f ahs1 ahs2 bhs1 bhs2 i j =
        merge_hs_slice_equal #_ #f ahs1 ahs2 bhs1 bhs2 (i + 1) j)
 
 val merge_hs_upd:
-  #hsz:pos -> #f:MTS.tag_fun_t #hsz ->
+  #hsz:pos -> #f:MTS.hash_fun_t #hsz ->
   hs1:hashess #hsz ->
   hs2:hashess #hsz {S.length hs1 = S.length hs2} ->
   i:nat{i < S.length hs1} ->
@@ -223,7 +223,7 @@ let rec merge_hs_upd #_ #f hs1 hs2 i v1 v2 =
   else merge_hs_upd #_ #f (S.tail hs1) (S.tail hs2) (i - 1) v1 v2
 
 val mt_olds_inv:
-  #hsz:pos -> #f:MTS.tag_fun_t #hsz ->
+  #hsz:pos -> #f:MTS.hash_fun_t #hsz ->
   lv:nat{lv <= 32} ->
   i:nat ->
   olds:hashess #hsz {S.length olds = 32} ->
@@ -235,7 +235,7 @@ let rec mt_olds_inv #_ #f lv i olds =
        mt_olds_inv #_ #f (lv + 1) (i / 2) olds)
 
 val mt_olds_inv_equiv:
-  #hsz:pos -> #f:MTS.tag_fun_t #hsz ->
+  #hsz:pos -> #f:MTS.hash_fun_t #hsz ->
   lv:nat{lv <= 32} ->
   i:nat ->
   olds1:hashess #hsz {S.length olds1 = 32} ->
@@ -250,7 +250,7 @@ let rec mt_olds_inv_equiv #hsz #f lv i olds1 olds2 =
        mt_olds_inv_equiv #_ #f (lv + 1) (i / 2) olds1 olds2)
 
 val mt_olds_hs_lth_inv_ok:
-  #hsz:pos -> #f:MTS.tag_fun_t #hsz ->
+  #hsz:pos -> #f:MTS.hash_fun_t #hsz ->
   lv:nat{lv <= 32} ->
   i:nat ->
   j:nat{i <= j /\ j < pow2 (32 - lv)} ->
@@ -264,7 +264,7 @@ let rec mt_olds_hs_lth_inv_ok #hsz #f lv i j olds hs =
   else (mt_olds_hs_lth_inv_ok #_ #f (lv + 1) (i / 2) (j / 2) olds hs)
 
 val mt_olds_hs_inv:
-  #hsz:pos -> #f:MTS.tag_fun_t #hsz ->
+  #hsz:pos -> #f:MTS.hash_fun_t #hsz ->
   lv:nat{lv < 32} ->
   i:nat ->
   j:nat{i <= j /\ j < pow2 (32 - lv)} ->
@@ -317,7 +317,7 @@ let rec log2c_bound n c =
   else log2c_bound (n / 2) (c - 1)
 
 val mt_hashes_lth_inv_log:
-  #hsz:pos -> #f:MTS.tag_fun_t #hsz ->
+  #hsz:pos -> #f:MTS.hash_fun_t #hsz ->
   j:nat ->
   fhs:hashess #hsz {S.length fhs = log2c j} ->
   GTot Type0 (decreases j)
@@ -329,7 +329,7 @@ let rec mt_hashes_lth_inv_log #_ #f j fhs =
 #push-options "--max_fuel 2"
 
 val mt_hashes_lth_inv_log_next:
-  #hsz:pos -> #f:MTS.tag_fun_t #hsz ->
+  #hsz:pos -> #f:MTS.hash_fun_t #hsz ->
   j:nat{j > 1} ->
   fhs:hashess #hsz {S.length fhs = log2c j} ->
   Lemma (requires mt_hashes_lth_inv_log #_ #f j fhs)
@@ -338,7 +338,7 @@ val mt_hashes_lth_inv_log_next:
 let mt_hashes_lth_inv_log_next #_ #_ _ _ = ()
 
 val mt_hashes_inv_log:
-  #hsz:pos -> #f:MTS.tag_fun_t #hsz ->
+  #hsz:pos -> #f:MTS.hash_fun_t #hsz ->
   j:nat ->
   fhs:hashess #hsz {S.length fhs = log2c j /\ mt_hashes_lth_inv_log #_ #f j fhs} ->
   GTot Type0 (decreases j)
@@ -348,7 +348,7 @@ let rec mt_hashes_inv_log #hsz #f j fhs =
        mt_hashes_inv_log #_ #f (j / 2) (S.tail fhs))
 
 val mt_hashes_lth_inv_log_converted_:
-  #hsz:pos -> #f:MTS.tag_fun_t #hsz ->
+  #hsz:pos -> #f:MTS.hash_fun_t #hsz ->
   lv:nat{lv <= 32} ->
   j:nat{j < pow2 (32 - lv)} ->
   fhs:hashess #hsz {S.length fhs = 32} ->
@@ -362,7 +362,7 @@ let rec mt_hashes_lth_inv_log_converted_ #_ #f lv j fhs =
        mt_hashes_lth_inv_log_converted_ #_ #f (lv + 1) (j / 2) fhs)
 
 val mt_hashes_lth_inv_log_converted:
-  #hsz:pos -> #f:MTS.tag_fun_t #hsz ->
+  #hsz:pos -> #f:MTS.hash_fun_t #hsz ->
   j:nat{j < pow2 32} ->
   fhs:hashess #hsz {S.length fhs = 32} ->
   Lemma (requires mt_hashes_lth_inv #hsz 0 j fhs)
@@ -372,7 +372,7 @@ let mt_hashes_lth_inv_log_converted #_ #f j fhs =
   mt_hashes_lth_inv_log_converted_ #_ #f 0 j fhs
 
 val mt_hashes_inv_log_converted_:
-  #hsz:pos -> #f:MTS.tag_fun_t #hsz ->
+  #hsz:pos -> #f:MTS.hash_fun_t #hsz ->
   lv:nat{lv <= 32} ->
   j:nat{j > 0 && j < pow2 (32 - lv)} ->
   fhs:hashess #hsz {S.length fhs = 32 /\ mt_hashes_lth_inv #hsz lv j fhs} ->
@@ -382,14 +382,16 @@ val mt_hashes_inv_log_converted_:
                   mt_hashes_inv_log #_ #f j (S.slice fhs lv (lv + log2c j))))
         (decreases j)
 #restart-solver
+#push-options "--z3rlimit 50 --initial_fuel 2 --max_fuel 2"
 let rec mt_hashes_inv_log_converted_ #_ #f lv j fhs =
   if j = 1 then ()
   else (log2c_bound (j / 2) (32 - (lv + 1));
         mt_hashes_lth_inv_log_converted_ #_ #f (lv + 1) (j / 2) fhs;
         mt_hashes_inv_log_converted_ #_ #f (lv + 1) (j / 2) fhs)
+#pop-options
 
 val mt_hashes_inv_log_converted:
-  #hsz:pos -> #f:MTS.tag_fun_t #hsz ->
+  #hsz:pos -> #f:MTS.hash_fun_t #hsz ->
   j:nat{j > 0 && j < pow2 32} ->
   fhs:hashess #hsz {S.length fhs = 32 /\ mt_hashes_lth_inv #hsz 0 j fhs} ->
   Lemma (requires mt_hashes_inv #_ #f 0 j fhs)
@@ -400,16 +402,16 @@ let mt_hashes_inv_log_converted #_ #f j fhs =
   mt_hashes_inv_log_converted_ #_ #f 0 j fhs
 
 val hash_seq_lift: 
-  #hsz:pos -> #f:MTS.tag_fun_t #hsz ->
+  #hsz:pos -> #f:MTS.hash_fun_t #hsz ->
   hs:hashes #hsz -> 
-  GTot (shs:MTS.tags #hsz {S.length shs = S.length hs})
+  GTot (shs:MTS.hashes #hsz {S.length shs = S.length hs})
        (decreases (S.length hs))
 let rec hash_seq_lift #_ #f hs =
   if S.length hs = 0 then S.empty
   else S.cons (MTS.HRaw (S.head hs)) (hash_seq_lift #_ #f (S.tail hs))
 
 val hash_seq_lift_index:
-  #hsz:pos -> #f:MTS.tag_fun_t #hsz ->
+  #hsz:pos -> #f:MTS.hash_fun_t #hsz ->
   hs:hashes #hsz ->
   Lemma (requires True)
         (ensures  forall (i:nat{i < S.length hs}).
@@ -421,11 +423,11 @@ let rec hash_seq_lift_index #_ #f hs =
 
 #pop-options // --max_fuel 2
 
-val create_pads: #hsz:pos -> len:nat -> GTot (pads:MTS.tags #hsz {S.length pads = len})
+val create_pads: #hsz:pos -> len:nat -> GTot (pads:MTS.hashes #hsz {S.length pads = len})
 let create_pads #hsz len = S.create len (MTS.HPad #hsz)
 
 val hash_seq_spec:
-  #hsz:pos -> #f:MTS.tag_fun_t #hsz ->
+  #hsz:pos -> #f:MTS.hash_fun_t #hsz ->
   hs:hashes #hsz {S.length hs > 0} ->
   GTot (smt:MTS.merkle_tree #hsz (log2c (S.length hs)))
 let hash_seq_spec #_ #f hs =
@@ -433,7 +435,7 @@ let hash_seq_spec #_ #f hs =
            (create_pads (pow2 (log2c (S.length hs)) - S.length hs))
 
 val hash_seq_spec_index_raw:
-  #hsz:pos -> #f:MTS.tag_fun_t #hsz ->
+  #hsz:pos -> #f:MTS.hash_fun_t #hsz ->
   hs:hashes #hsz {S.length hs > 0} ->
   i:nat{i < S.length hs} ->
   Lemma (S.index (hash_seq_spec #_ #f hs) i == MTS.HRaw #hsz (S.index hs i))
@@ -443,7 +445,7 @@ let hash_seq_spec_index_raw #_ #f hs i =
 // Now about recovering rightmost hashes
 
 val mt_hashes_next_rel_lift_even:
-  #hsz:pos -> #f:MTS.tag_fun_t #hsz ->
+  #hsz:pos -> #f:MTS.hash_fun_t #hsz ->
   j:nat{j > 1} ->
   hs:hashes #hsz {S.length hs = j} ->
   nhs:hashes #hsz {S.length nhs = j / 2} ->
@@ -455,7 +457,7 @@ let mt_hashes_next_rel_lift_even #_ #f j hs nhs =
   hash_seq_lift_index #_ #f nhs
 
 val mt_hashes_next_rel_lift_odd:
-  #hsz:pos -> #f:MTS.tag_fun_t #hsz ->
+  #hsz:pos -> #f:MTS.hash_fun_t #hsz ->
   j:nat{j > 1} ->
   hs:hashes #hsz {S.length hs = j} ->
   nhs:hashes #hsz {S.length nhs = j / 2} ->
@@ -470,7 +472,7 @@ let mt_hashes_next_rel_lift_odd #_ #f j hs nhs =
   hash_seq_lift_index #_ #f nhs
 
 val mt_hashes_next_rel_next_even:
-  #hsz:pos -> #f:MTS.tag_fun_t #hsz ->
+  #hsz:pos -> #f:MTS.hash_fun_t #hsz ->
   j:nat{j > 1} ->
   hs:hashes #hsz {S.length hs = j} ->
   nhs:hashes #hsz {S.length nhs = j / 2} ->
@@ -484,7 +486,7 @@ let mt_hashes_next_rel_next_even #_ #f j hs nhs =
     (hash_seq_spec #_ #f hs) (hash_seq_spec #_ #f nhs)
 
 val hash_seq_spec_full:
-  #hsz:pos -> #f:MTS.tag_fun_t #hsz ->
+  #hsz:pos -> #f:MTS.hash_fun_t #hsz ->
   hs:hashes #hsz {S.length hs > 0} ->
   acc:hash #hsz -> actd:bool ->
   GTot (smt:MTS.merkle_tree #hsz (log2c (S.length hs)))
@@ -494,7 +496,7 @@ let hash_seq_spec_full #_ #f hs acc actd =
   else hash_seq_spec #_ #f hs
 
 val hash_seq_spec_full_index_raw:
-  #hsz:pos -> #f:MTS.tag_fun_t #hsz ->
+  #hsz:pos -> #f:MTS.hash_fun_t #hsz ->
   hs:hashes #hsz {S.length hs > 0} ->
   acc:hash #hsz -> actd:bool -> i:nat{i < S.length hs} ->
   Lemma (S.index (hash_seq_spec_full #_ #f hs acc actd) i ==
@@ -503,13 +505,13 @@ let hash_seq_spec_full_index_raw #_ #f hs acc actd i =
   hash_seq_spec_index_raw #_ #f hs i
 
 val hash_seq_spec_full_case_true:
-  #hsz:pos -> #f:MTS.tag_fun_t #hsz ->
+  #hsz:pos -> #f:MTS.hash_fun_t #hsz ->
   hs:hashes #hsz {S.length hs > 0} -> acc:hash #hsz ->
   Lemma (S.index (hash_seq_spec_full #_ #f hs acc true) (S.length hs) == MTS.HRaw acc)
 let hash_seq_spec_full_case_true #_ #_ _ _ = ()  
 
 val hash_seq_spec_full_even_next:
-  #hsz:pos -> #f:MTS.tag_fun_t #hsz ->
+  #hsz:pos -> #f:MTS.hash_fun_t #hsz ->
   j:nat{j > 0} ->
   hs:hashes #hsz {S.length hs = j} ->
   nhs:hashes #hsz {S.length nhs = j / 2} ->
@@ -538,7 +540,7 @@ let hash_seq_spec_full_even_next #_ #f j hs nhs acc actd =
 
 #push-options "--z3rlimit 80"
 val hash_seq_spec_full_odd_next:
-  #hsz:pos -> #f:MTS.tag_fun_t #hsz ->
+  #hsz:pos -> #f:MTS.hash_fun_t #hsz ->
   j:nat{j > 1} ->
   hs:hashes #hsz {S.length hs = j} ->
   nhs:hashes #hsz {S.length nhs = j / 2} ->
@@ -569,7 +571,7 @@ let hash_seq_spec_full_odd_next #_ #f j hs nhs acc actd nacc =
 #pop-options
 
 val hash_seq_spec_full_next:
-  #hsz:pos -> #f:MTS.tag_fun_t #hsz ->
+  #hsz:pos -> #f:MTS.hash_fun_t #hsz ->
   j:nat{j > 1} ->
   hs:hashes #hsz {S.length hs = j} ->
   nhs:hashes #hsz {S.length nhs = j / 2} ->
@@ -589,7 +591,7 @@ let hash_seq_spec_full_next #_ #f j hs nhs acc actd nacc nactd =
   else hash_seq_spec_full_odd_next #_ #f j hs nhs acc actd nacc
 
 val mt_rhs_inv:
-  #hsz:pos -> #f:MTS.tag_fun_t #hsz ->
+  #hsz:pos -> #f:MTS.hash_fun_t #hsz ->
   j:nat ->
   smt:MTS.merkle_tree #hsz (log2c j) ->
   rhs:hashes #hsz {S.length rhs = log2c j} ->
@@ -606,7 +608,7 @@ let rec mt_rhs_inv #_ #f j smt rhs actd =
   end
 
 val mt_root_inv:
-  #hsz:pos -> #f:MTS.tag_fun_t #hsz ->
+  #hsz:pos -> #f:MTS.hash_fun_t #hsz ->
   hs0:hashes #hsz {S.length hs0 > 0} ->
   acc:hash #hsz -> actd:bool ->
   rt:hash #hsz ->
@@ -618,32 +620,32 @@ let mt_root_inv #_ #f hs0 acc actd rt =
 val mt_base:
   #hsz:pos -> 
   mt:merkle_tree #hsz {mt_wf_elts mt} ->
-  olds:hashess #hsz {S.length olds = 32 /\ mt_olds_inv #_ #(MT?.tag_fun mt) 0 (MT?.i mt) olds} ->
+  olds:hashess #hsz {S.length olds = 32 /\ mt_olds_inv #_ #(MT?.hash_fun mt) 0 (MT?.i mt) olds} ->
   GTot (bhs:hashes #hsz {S.length bhs = MT?.j mt})
 let mt_base #hsz mt olds =
-  S.head (merge_hs #hsz #(MT?.tag_fun mt) olds (MT?.hs mt))
+  S.head (merge_hs #hsz #(MT?.hash_fun mt) olds (MT?.hs mt))
 
 #pop-options // --max_fuel 1
 
 val mt_spec:
   #hsz:pos -> 
   mt:merkle_tree #hsz {mt_wf_elts mt /\ MT?.j mt > 0} ->
-  olds:hashess{S.length olds = 32 /\ mt_olds_inv #hsz #(MT?.tag_fun mt) 0 (MT?.i mt) olds} ->
+  olds:hashess{S.length olds = 32 /\ mt_olds_inv #hsz #(MT?.hash_fun mt) 0 (MT?.i mt) olds} ->
   GTot (smt:MTS.merkle_tree #hsz (log2c (MT?.j mt)))
 let mt_spec #hsz mt olds =
-  hash_seq_spec #_ #(MT?.tag_fun mt) (mt_base mt olds)
+  hash_seq_spec #_ #(MT?.hash_fun mt) (mt_base mt olds)
 
 val mt_inv: 
   #hsz:pos -> 
   mt:merkle_tree #hsz {mt_wf_elts mt} ->
-  olds:hashess{S.length olds = 32 /\ mt_olds_inv #_ #(MT?.tag_fun mt) 0 (MT?.i mt) olds} ->
+  olds:hashess{S.length olds = 32 /\ mt_olds_inv #_ #(MT?.hash_fun mt) 0 (MT?.i mt) olds} ->
   GTot Type0
 let mt_inv #hsz mt olds =
   let i = MT?.i mt in
   let j = MT?.j mt in
   let hs = MT?.hs mt in
   let rhs = MT?.rhs mt in
-  let f = MT?.tag_fun mt in
+  let f = MT?.hash_fun mt in
   let fhs = merge_hs #hsz #f olds hs in
   let rt = MT?.mroot mt in
   log2c_bound j 32;
