secure_api/merkle_tree/MerkleTree.Spec.fst
@@ -10,11 +10,11 @@ module S = FStar.Seq
 
 // For SHA2_256, this is is a sequence of 32 bytes
 // These are secret bytes, hence not an eqtype
-type tag (#hsz:pos) = b:Spec.Hash.Definitions.bytes { Seq.length b = hsz }
+type hash (#hsz:pos) = b:Spec.Hash.Definitions.bytes { Seq.length b = hsz }
 
-type tag_fun_t (#hsz:pos) = tag #hsz -> tag #hsz -> GTot (tag #hsz)
+type hash_fun_t (#hsz:pos) = hash #hsz -> hash #hsz -> GTot (hash #hsz)
 
-val sha256_compress: tag_fun_t #32
+val sha256_compress: hash_fun_t #32
 let sha256_compress src1 src2 =
   let sz = Spec.Hash.Definitions.SHA2_256 in
   let hash_alg = Spec.Hash.Definitions.SHA2_256 in
@@ -25,32 +25,32 @@ let sha256_compress src1 src2 =
 /// For simplicity, we will specify the root for a sequence of [i]
 /// tags where [i <= 2^n] as the root of a full binary tree with [2^n]
 /// leaves obtained by padding the sequence with dummies. This
-/// requires extending the definitions of tags and tages. Our
-/// extended definition of tag justifies skipping any concrete
+/// requires extending the definitions of hashes and hash functions. Our
+/// extended definition of hash justifies skipping any concrete
 /// computation on dummies.
 noeq
-type padded_tag #hsz =
-| HRaw: hr:tag #hsz -> padded_tag #hsz
+type padded_hash #hsz =
+| HRaw: hr:hash #hsz -> padded_hash #hsz
 | HPad // right padding to make the size of a Merkle tree a power of 2
 
-val padded_tag_fun: (#hsz:pos) -> (f:tag_fun_t #hsz) -> (lh:padded_tag #hsz) -> (rh:padded_tag #hsz) -> GTot (padded_tag #hsz)
-let padded_tag_fun #hsz f lh rh =
-  allow_inversion (padded_tag #hsz);
+val padded_hash_fun: (#hsz:pos) -> (f:hash_fun_t #hsz) -> (lh:padded_hash #hsz) -> (rh:padded_hash #hsz) -> GTot (padded_hash #hsz)
+let padded_hash_fun #hsz f lh rh =
+  allow_inversion (padded_hash #hsz);
   match lh, rh with
   | HPad    , _        -> HPad
   | _       , HPad     -> lh
   | HRaw lhr, HRaw rhr -> HRaw (f lhr rhr)
 
 noextract
-val tags (#hsz:pos): Type0
-let tags #hsz = S.seq (padded_tag #hsz)
+val hashes (#hsz:pos): Type0
+let hashes #hsz = S.seq (padded_hash #hsz)
 
-type merkle_tree (#hsz:pos) n = hs:tags #hsz {S.length hs = pow2 n}
+type merkle_tree (#hsz:pos) n = hs:hashes #hsz {S.length hs = pow2 n}
 
-val mt_get: #hsz:pos -> #n:nat -> mt:merkle_tree #hsz n -> idx:nat{idx < pow2 n} -> GTot (padded_tag #hsz)
+val mt_get: #hsz:pos -> #n:nat -> mt:merkle_tree #hsz n -> idx:nat{idx < pow2 n} -> GTot (padded_hash #hsz)
 let mt_get #_ #_ mt idx = S.index mt idx
 
-unfold let op_String_Access (#hsz:pos) = S.index #(padded_tag #hsz)
+unfold let op_String_Access (#hsz:pos) = S.index #(padded_hash #hsz)
 
 #push-options "--max_fuel 1"
 
@@ -64,22 +64,22 @@ val mt_left_right: #hsz:pos -> #n:pos -> mt:merkle_tree #hsz n ->
   Lemma (S.equal mt (mt_left mt @| mt_right mt))
 let mt_left_right #_ #_ mt = ()
 
-val hs_next_lv: #hsz:pos -> #f:tag_fun_t #hsz -> #n:nat -> hs:tags #hsz {S.length hs = 2 * n} -> GTot (nhs:tags #hsz {S.length nhs = n})
+val hs_next_lv: #hsz:pos -> #f:hash_fun_t #hsz -> #n:nat -> hs:hashes #hsz {S.length hs = 2 * n} -> GTot (nhs:hashes #hsz {S.length nhs = n})
 let rec hs_next_lv #hsz #f #n hs =
   if n = 0 then S.empty
   else S.cons
-    (padded_tag_fun #hsz f hs.[0] hs.[1])
+    (padded_hash_fun #hsz f hs.[0] hs.[1])
     (hs_next_lv #hsz #f #(n-1) (S.slice hs 2 (S.length hs)))
 
-val hs_next_lv_index: #hsz:pos -> #f:tag_fun_t #hsz -> #n:nat  -> hs:tags{S.length hs = 2 * n} -> i:nat{i < n} ->
-  Lemma ((hs_next_lv #hsz #f #n hs).[i] == padded_tag_fun #hsz f hs.[2 * i] hs.[2 * i + 1])
+val hs_next_lv_index: #hsz:pos -> #f:hash_fun_t #hsz -> #n:nat  -> hs:hashes{S.length hs = 2 * n} -> i:nat{i < n} ->
+  Lemma ((hs_next_lv #hsz #f #n hs).[i] == padded_hash_fun #hsz f hs.[2 * i] hs.[2 * i + 1])
 let rec hs_next_lv_index #hsz #f #n hs i =
   if n = 0 || i = 0 then ()
   else hs_next_lv_index #hsz #f #(n - 1) (S.slice hs 2 (S.length hs)) (i - 1)
 
 val hs_next_lv_slice:
-  #hsz:pos -> #f:tag_fun_t #hsz -> #n:nat  ->
-  hs:tags{S.length hs = 2 * n} -> i:nat -> j:nat{i <= j && j <= n} ->
+  #hsz:pos -> #f:hash_fun_t #hsz -> #n:nat  ->
+  hs:hashes{S.length hs = 2 * n} -> i:nat -> j:nat{i <= j && j <= n} ->
   Lemma (requires True)
         (ensures  S.equal (hs_next_lv #hsz #f #(j - i) (S.slice hs (2 * i) (2 * j)))
                           (S.slice (hs_next_lv #hsz #f #n hs) i j))
@@ -89,30 +89,30 @@ let rec hs_next_lv_slice #hsz #f #n hs i j =
   else begin
     let x = S.slice hs (2 * i) (2 * j) in
     assert (S.equal (hs_next_lv #hsz #f #(j - i) x)
-                    (S.cons (padded_tag_fun #hsz f x.[0] x.[1])
+                    (S.cons (padded_hash_fun #hsz f x.[0] x.[1])
                             (hs_next_lv #hsz #f #(j - i - 1) (S.slice x 2 (S.length x)))));
     hs_next_lv_slice #hsz #f #n hs (i + 1) j;
     hs_next_lv_index #hsz #f #n hs i
   end
 
-val mt_next_lv: #hsz:pos -> #f:tag_fun_t #hsz -> #n:pos -> mt:merkle_tree #hsz n -> GTot (merkle_tree #hsz (n-1))
+val mt_next_lv: #hsz:pos -> #f:hash_fun_t #hsz -> #n:pos -> mt:merkle_tree #hsz n -> GTot (merkle_tree #hsz (n-1))
 let mt_next_lv #_ #f #n mt = hs_next_lv #_ #f #(pow2 (n-1)) mt
 
-val mt_next_lv_mt_left: #hsz:pos -> #f:tag_fun_t #hsz -> #n:nat{1 < n} -> mt:merkle_tree #hsz n ->
+val mt_next_lv_mt_left: #hsz:pos -> #f:hash_fun_t #hsz -> #n:nat{1 < n} -> mt:merkle_tree #hsz n ->
   Lemma (S.equal (mt_next_lv #_ #f #_ (mt_left mt)) (mt_left (mt_next_lv #_ #f #_ mt)))
 let mt_next_lv_mt_left #hsz #f #n mt =
   hs_next_lv_slice #_ #f #(pow2 (n-1)) mt 0 (pow2 (n-2))
 
-val mt_next_lv_mt_right: #hsz:pos -> #f:tag_fun_t #hsz -> #n:nat{1 < n} -> mt:merkle_tree #hsz n ->
+val mt_next_lv_mt_right: #hsz:pos -> #f:hash_fun_t #hsz -> #n:nat{1 < n} -> mt:merkle_tree #hsz n ->
   Lemma (S.equal (mt_next_lv #_ #f #_ (mt_right mt)) (mt_right (mt_next_lv #_ #f #_ mt)))
 let mt_next_lv_mt_right #hsz #f #n mt =
   hs_next_lv_slice #hsz #f #(pow2 (n-1)) mt (pow2 (n-2)) (pow2 (n-1))
 
 val hs_next_lv_equiv:
-  #hsz:pos -> #f:tag_fun_t #hsz ->
+  #hsz:pos -> #f:hash_fun_t #hsz ->
   j:nat -> n:pos{j <= 2 * n} ->
-  hs1:tags{S.length hs1 = 2 * n} ->
-  hs2:tags{S.length hs2 = 2 * n} ->
+  hs1:hashes{S.length hs1 = 2 * n} ->
+  hs2:hashes{S.length hs2 = 2 * n} ->
   Lemma (requires S.equal (S.slice hs1 0 j) (S.slice hs2 0 j))
         (ensures  S.equal (S.slice (hs_next_lv #hsz #f #n hs1) 0 (j / 2))
                           (S.slice (hs_next_lv #hsz #f #n hs2) 0 (j / 2)))
@@ -121,8 +121,8 @@ let hs_next_lv_equiv #hsz #f j n hs1 hs2 =
   forall_intro (hs_next_lv_index #_ #f #n hs2);
   let hs1' = hs_next_lv #_ #f #n hs1 in
   let hs2' = hs_next_lv #_ #f #n hs2 in
-  assert (forall (i:nat{i < j / 2}). hs1'.[i] == padded_tag_fun #hsz f hs1.[2 * i] hs1.[2 * i + 1]);
-  assert (forall (i:nat{i < j / 2}). hs2'.[i] == padded_tag_fun #hsz f hs2.[2 * i] hs2.[2 * i + 1]);
+  assert (forall (i:nat{i < j / 2}). hs1'.[i] == padded_hash_fun #hsz f hs1.[2 * i] hs1.[2 * i + 1]);
+  assert (forall (i:nat{i < j / 2}). hs2'.[i] == padded_hash_fun #hsz f hs2.[2 * i] hs2.[2 * i + 1]);
   assert (forall (i:nat{i < j}).     (S.slice hs1 0 j).[i] == (S.slice hs2 0 j).[i]);
   assert (forall (i:nat{i < j}).     hs1.[i] == hs2.[i]);
   assert (forall (i:nat{i < j / 2}). hs1.[2 * i] == hs2.[2 * i]);
@@ -130,7 +130,7 @@ let hs_next_lv_equiv #hsz #f j n hs1 hs2 =
   assert (forall (i:nat{i < j / 2}). hs1'.[i] == hs2'.[i])
 
 val mt_next_lv_equiv:
-  #hsz:pos -> #f:tag_fun_t #hsz ->
+  #hsz:pos -> #f:hash_fun_t #hsz ->
   j:nat -> n:pos{j <= pow2 n} ->
   mt1:merkle_tree #hsz n -> mt2:merkle_tree #hsz n ->
   Lemma (requires S.equal (S.slice mt1 0 j) (S.slice mt2 0 j))
@@ -140,18 +140,18 @@ let mt_next_lv_equiv #hsz #f j n mt1 mt2 =
   hs_next_lv_equiv #_ #f j (pow2 (n-1)) mt1 mt2
 
 val hs_next_rel:
-  #hsz:pos -> #f:tag_fun_t #hsz ->
+  #hsz:pos -> #f:hash_fun_t #hsz ->
   n:nat ->
-  hs:tags #hsz {S.length hs = 2 * n} ->
-  nhs:tags #hsz {S.length nhs = n} ->
+  hs:hashes #hsz {S.length hs = 2 * n} ->
+  nhs:hashes #hsz {S.length nhs = n} ->
   GTot Type0
 let hs_next_rel #hsz #f n hs nhs =
   forall (i:nat{i < n}).
     S.index nhs i ==
-    padded_tag_fun #hsz f (S.index hs (2 * i)) (S.index hs (2 * i + 1))
+    padded_hash_fun #hsz f (S.index hs (2 * i)) (S.index hs (2 * i + 1))
 
 val mt_next_rel:
-  #hsz:pos -> #f:tag_fun_t #hsz ->
+  #hsz:pos -> #f:hash_fun_t #hsz ->
   n:pos ->
   mt:merkle_tree #hsz n ->
   nmt:merkle_tree #hsz (n - 1) ->
@@ -160,10 +160,10 @@ let mt_next_rel #hsz #f n mt nmt =
   hs_next_rel #hsz #f (pow2 (n-1)) mt nmt
 
 val hs_next_rel_next_lv:
-  #hsz:pos -> #f:tag_fun_t #hsz ->
+  #hsz:pos -> #f:hash_fun_t #hsz ->
   n:nat ->
-  hs:tags{S.length hs = 2 * n} ->
-  nhs:tags{S.length nhs = n} ->
+  hs:hashes{S.length hs = 2 * n} ->
+  nhs:hashes{S.length nhs = n} ->
   Lemma (requires hs_next_rel #_ #f n hs nhs)
         (ensures  S.equal nhs (hs_next_lv #_ #f #n hs))
 let rec hs_next_rel_next_lv #hsz #f n hs nhs =
@@ -173,7 +173,7 @@ let rec hs_next_rel_next_lv #hsz #f n hs nhs =
          (S.slice nhs 1 (S.length nhs))
 
 val mt_next_rel_next_lv:
-  #hsz:pos -> #f:tag_fun_t #hsz ->
+  #hsz:pos -> #f:hash_fun_t #hsz ->
   n:pos ->
   mt:merkle_tree #hsz n ->
   nmt:merkle_tree (n - 1) ->
@@ -183,57 +183,57 @@ let mt_next_rel_next_lv #hsz #f n mt nmt =
   hs_next_rel_next_lv #_ #f (pow2 (n-1)) mt nmt
 
 val mt_next_rel_upd_even:
-  #hsz:pos -> #f:tag_fun_t #hsz ->
+  #hsz:pos -> #f:hash_fun_t #hsz ->
   n:pos ->
   mt:merkle_tree #hsz n ->
   nmt:merkle_tree (n - 1) ->
   i:nat{i < pow2 (n-1)} -> 
-  v:padded_tag ->
+  v:padded_hash ->
   Lemma (requires mt_next_rel #_ #f n mt nmt)
         (ensures  mt_next_rel #_ #f n
                    (S.upd mt (2 * i) v)
-                   (S.upd nmt i (padded_tag_fun #hsz f v (S.index mt (2 * i + 1)))))
+                   (S.upd nmt i (padded_hash_fun #hsz f v (S.index mt (2 * i + 1)))))
 let mt_next_rel_upd_even #hsz #f n mt nmt i v = ()
 
 #push-options "--z3rlimit 10 --initial_fuel 1 --max_fuel 1 --initial_ifuel 1 --max_ifuel 1"
 val mt_next_rel_upd_even_pad:
-  #hsz:pos -> #f:tag_fun_t #hsz ->
+  #hsz:pos -> #f:hash_fun_t #hsz ->
   n:pos ->
   mt:merkle_tree #hsz n ->
   nmt:merkle_tree #hsz (n - 1) ->
   i:nat{i < pow2 (n-1)} -> 
-  v:padded_tag #hsz ->
+  v:padded_hash #hsz ->
   Lemma (requires (mt_next_rel #_ #f n mt nmt) /\ (S.index mt (2 * i + 1) == HPad))
         (ensures (mt_next_rel #_ #f n (S.upd mt (2 * i) v) (S.upd nmt i v)))
 let mt_next_rel_upd_even_pad #hsz #f n mt nmt i v = ()
 #pop-options
 
 val mt_next_rel_upd_odd:
-  #hsz:pos -> #f:tag_fun_t #hsz ->
+  #hsz:pos -> #f:hash_fun_t #hsz ->
   n:pos ->
   mt:merkle_tree #hsz n ->
   nmt:merkle_tree (n - 1) ->
   i:nat{i < pow2 (n-1)} -> 
-  v:padded_tag ->
+  v:padded_hash ->
   Lemma (requires mt_next_rel #_ #f n mt nmt)
         (ensures  mt_next_rel #_ #f n
                    (S.upd mt (2 * i + 1) v)
-                   (S.upd nmt i (padded_tag_fun #_ f (S.index mt (2 * i)) v)))
+                   (S.upd nmt i (padded_hash_fun #_ f (S.index mt (2 * i)) v)))
 let mt_next_rel_upd_odd #hsz #f n mt nmt i v = ()
 
 // fournet: just [root]?
 val mt_get_root: 
-  #hsz:pos -> #f:tag_fun_t #hsz ->
-  #n:nat -> mt:merkle_tree #hsz n -> GTot (padded_tag #hsz)
+  #hsz:pos -> #f:hash_fun_t #hsz ->
+  #n:nat -> mt:merkle_tree #hsz n -> GTot (padded_hash #hsz)
 let rec mt_get_root #hsz #f #n mt =
   if n = 0 then mt.[0]
   else mt_get_root #_ #f (mt_next_lv #_ #f mt)
 
 #push-options "--initial_fuel 2 --max_fuel 2"
 
-val mt_get_root_step: #hsz:pos -> #f:tag_fun_t #hsz -> #n:pos -> mt:merkle_tree #hsz n ->
+val mt_get_root_step: #hsz:pos -> #f:hash_fun_t #hsz -> #n:pos -> mt:merkle_tree #hsz n ->
   Lemma (mt_get_root #_ #f mt ==
-         padded_tag_fun #_ f (mt_get_root #_ #f (mt_left mt)) (mt_get_root #_ #f (mt_right mt)))
+         padded_hash_fun #_ f (mt_get_root #_ #f (mt_left mt)) (mt_get_root #_ #f (mt_right mt)))
 let rec mt_get_root_step #hsz #f #n mt =
   if n = 1 then ()
   else begin
@@ -244,13 +244,13 @@ let rec mt_get_root_step #hsz #f #n mt =
 
 #pop-options
 
-type merkle_path #hsz n = S.lseq (padded_tag #hsz) n
+type path #hsz n = S.lseq (padded_hash #hsz) n
 
 /// We first specify full paths, including padding.
 
 val mt_get_path: 
-  #hsz:pos -> #f:tag_fun_t #hsz -> #n:nat -> 
-  mt:merkle_tree #hsz n -> i:nat{i < pow2 n} -> GTot (merkle_path #hsz n)
+  #hsz:pos -> #f:hash_fun_t #hsz -> #n:nat -> 
+  mt:merkle_tree #hsz n -> i:nat{i < pow2 n} -> GTot (path #hsz n)
 let rec mt_get_path #hsz #f #n t i =
   if n = 0 then S.empty
   else S.cons
@@ -258,18 +258,18 @@ let rec mt_get_path #hsz #f #n t i =
     (mt_get_path #_ #f (mt_next_lv #_ #f t) (i / 2))
 
 val mt_verify_: 
-  #hsz:pos -> #f:tag_fun_t #hsz ->#n:nat -> 
-  p:merkle_path #hsz n -> idx:nat{idx < pow2 n} -> padded_tag #hsz -> GTot (padded_tag #hsz)
+  #hsz:pos -> #f:hash_fun_t #hsz ->#n:nat -> 
+  p:path #hsz n -> idx:nat{idx < pow2 n} -> padded_hash #hsz -> GTot (padded_hash #hsz)
 let rec mt_verify_ #hsz #f #n p idx h =
   if n = 0 then h
   else mt_verify_ #_ #f #(n-1) (S.tail p) (idx / 2)
                   (if idx % 2 = 0
-                   then padded_tag_fun #_ f h (S.head p)
-                   else padded_tag_fun #_ f (S.head p) h)
+                   then padded_hash_fun #_ f h (S.head p)
+                   else padded_hash_fun #_ f (S.head p) h)
 
 val mt_verify: 
-  #hsz:pos -> #f:tag_fun_t #hsz -> #n:nat -> 
-  p:(merkle_path #hsz n) -> idx:nat{idx < pow2 n} -> padded_tag #hsz -> padded_tag #hsz -> GTot prop
+  #hsz:pos -> #f:hash_fun_t #hsz -> #n:nat -> 
+  p:(path #hsz n) -> idx:nat{idx < pow2 n} -> padded_hash #hsz -> padded_hash #hsz -> GTot prop
 let mt_verify #hsz #f #n p idx h rt =
   rt == mt_verify_ #_ #f p idx h
 
@@ -277,29 +277,29 @@ let mt_verify #hsz #f #n p idx h rt =
 /// Correctness: the root of a tree is correctly recomputed from any of its paths
 
 val hs_next_lv_get: 
-  #hsz:pos -> #f:tag_fun_t #hsz -> #n:pos -> 
-  hs:tags{S.length hs = 2 * n} -> idx:nat{idx < 2 * n} ->
+  #hsz:pos -> #f:hash_fun_t #hsz -> #n:pos -> 
+  hs:hashes{S.length hs = 2 * n} -> idx:nat{idx < 2 * n} ->
   Lemma ((hs_next_lv #_ #f #n hs).[idx / 2] ==
          (if idx % 2 = 0
-          then padded_tag_fun #_ f hs.[idx] hs.[idx + 1]
-          else padded_tag_fun #_ f hs.[idx - 1] hs.[idx]))
+          then padded_hash_fun #_ f hs.[idx] hs.[idx + 1]
+          else padded_hash_fun #_ f hs.[idx - 1] hs.[idx]))
 let rec hs_next_lv_get #hsz #f #n hs idx =
   if idx < 2 then ()
   else hs_next_lv_get #_ #f #(n-1) (S.slice hs 2 (S.length hs)) (idx - 2)
 
 val mt_next_lv_get: 
-  #hsz:pos -> #f:tag_fun_t #hsz -> #n:pos -> 
+  #hsz:pos -> #f:hash_fun_t #hsz -> #n:pos -> 
   mt:merkle_tree #hsz n -> idx:nat{idx < pow2 n} ->
   Lemma (
      (mt_next_lv #_ #f mt).[idx / 2] ==
      (if idx % 2 = 0
-      then padded_tag_fun #_ f mt.[idx] mt.[idx + 1]
-      else padded_tag_fun #_ f mt.[idx - 1] mt.[idx]))
+      then padded_hash_fun #_ f mt.[idx] mt.[idx + 1]
+      else padded_hash_fun #_ f mt.[idx - 1] mt.[idx]))
 let mt_next_lv_get #hsz #f #n mt idx =
   hs_next_lv_get #_ #f #(pow2 (n-1)) mt idx
 
 val mt_get_path_ok_: 
-  #hsz:pos -> #f:tag_fun_t #hsz -> #n:nat -> 
+  #hsz:pos -> #f:hash_fun_t #hsz -> #n:nat -> 
   t:merkle_tree #hsz n -> i:nat{i < pow2 n} ->
   Lemma (mt_verify_ #_ #f (mt_get_path #_ #f t i) i (mt_get t i) == mt_get_root #_ #f t)
 let rec mt_get_path_ok_ #hsz #f #n mt idx =
@@ -314,7 +314,7 @@ let rec mt_get_path_ok_ #hsz #f #n mt idx =
   end
 
 
-/// Security: we reduce tree collisions to collisions on the tag
+/// Security: we reduce tree collisions to collisions on the hash
 /// compression function. Such collisions yield collisions on the SHA2
 /// standard (by adding the same length and padding to the
 /// accumulators).
@@ -322,130 +322,130 @@ let rec mt_get_path_ok_ #hsz #f #n mt idx =
 /// One complication addressed in the proof is the handling of
 /// implicit padding.
 
-/// All tages in a sequence are raw tages, not padding
-val raw_tages: 
-  #hsz:pos -> #f:tag_fun_t #hsz ->
-  hs:tags #hsz -> Tot Type0 (decreases (S.length hs))
-let rec raw_tages #hsz #f hs =
+/// All hashes in a sequence are raw hashes, not padding
+val raw_hashes: 
+  #hsz:pos -> #f:hash_fun_t #hsz ->
+  hs:hashes #hsz -> Tot Type0 (decreases (S.length hs))
+let rec raw_hashes #hsz #f hs =
   if S.length hs = 0 then True
-  else (HRaw? (S.head hs) /\ raw_tages #_ #f (S.tail hs))
+  else (HRaw? (S.head hs) /\ raw_hashes #_ #f (S.tail hs))
 
-val raw_tages_raws: 
-  #hsz:pos -> #f:tag_fun_t #hsz ->
-  hs:tags{raw_tages #hsz #f hs} ->
-  Tot (S.seq (tag #hsz)) (decreases (S.length hs))
-let rec raw_tages_raws #hsz #f hs =
+val raw_hashes_raws: 
+  #hsz:pos -> #f:hash_fun_t #hsz ->
+  hs:hashes{raw_hashes #hsz #f hs} ->
+  Tot (S.seq (hash #hsz)) (decreases (S.length hs))
+let rec raw_hashes_raws #hsz #f hs =
   if S.length hs = 0 then S.empty
-  else S.cons (HRaw?.hr (S.head hs)) (raw_tages_raws #_ #f (S.tail hs))
+  else S.cons (HRaw?.hr (S.head hs)) (raw_hashes_raws #_ #f (S.tail hs))
 
-val raw_tages_index:
-  #hsz:pos -> #f:tag_fun_t #hsz ->
-  hs:tags -> i:nat{i < S.length hs} ->
-  Lemma (requires raw_tages #_ #f hs)
+val raw_hashes_index:
+  #hsz:pos -> #f:hash_fun_t #hsz ->
+  hs:hashes -> i:nat{i < S.length hs} ->
+  Lemma (requires raw_hashes #_ #f hs)
         (ensures HRaw? #hsz hs.[i])
         (decreases i)
-let rec raw_tages_index #hsz #f hs i =
+let rec raw_hashes_index #hsz #f hs i =
   if i = 0 then ()
-  else raw_tages_index #_ #f (S.tail hs) (i - 1)
+  else raw_hashes_index #_ #f (S.tail hs) (i - 1)
 
-val raw_tages_slice:
-  #hsz:pos -> #f:tag_fun_t #hsz ->
-  hs:tags -> i:nat -> j:nat{i <= j && j <= S.length hs} ->
-  Lemma (requires raw_tages #_ #f hs)
-        (ensures  raw_tages #_ #f (S.slice hs i j))
+val raw_hashes_slice:
+  #hsz:pos -> #f:hash_fun_t #hsz ->
+  hs:hashes -> i:nat -> j:nat{i <= j && j <= S.length hs} ->
+  Lemma (requires raw_hashes #_ #f hs)
+        (ensures  raw_hashes #_ #f (S.slice hs i j))
         (decreases (j - i))
-let rec raw_tages_slice #hsz #f hs i j =
+let rec raw_hashes_slice #hsz #f hs i j =
   if i = j then ()
   else (
-    raw_tages_index #_ #f hs i;
-    raw_tages_slice #_ #f hs (i + 1) j)
+    raw_hashes_index #_ #f hs i;
+    raw_hashes_slice #_ #f hs (i + 1) j)
 
-/// All tages in a sequence are just padding
-val pad_tages: 
-  #hsz:pos -> #f:tag_fun_t #hsz ->
-  hs:tags #hsz -> Type0
-let pad_tages #hsz #f hs =
+/// All hashes in a sequence are just padding
+val pad_hashes: 
+  #hsz:pos -> #f:hash_fun_t #hsz ->
+  hs:hashes #hsz -> Type0
+let pad_hashes #hsz #f hs =
   S.equal hs (S.create (S.length hs) HPad)
 
-val pad_tages_slice:
-  #hsz:pos -> #f:tag_fun_t #hsz ->
-  hs:tags -> i:nat -> j:nat{i <= j && j <= S.length hs} ->
-  Lemma (requires pad_tages #_ #f hs)
-        (ensures  pad_tages #_ #f (S.slice hs i j))
+val pad_hashes_slice:
+  #hsz:pos -> #f:hash_fun_t #hsz ->
+  hs:hashes -> i:nat -> j:nat{i <= j && j <= S.length hs} ->
+  Lemma (requires pad_hashes #_ #f hs)
+        (ensures  pad_hashes #_ #f (S.slice hs i j))
         (decreases (j - i))
-let rec pad_tages_slice #hsz #f hs i j =
+let rec pad_hashes_slice #hsz #f hs i j =
   if i = j then ()
-  else pad_tages_slice #_ #f hs (i + 1) j
+  else pad_hashes_slice #_ #f hs (i + 1) j
 
 /// Right-padded Merkle tree, a tree refinement
 
-let rpmt (#hsz:pos) (#f:tag_fun_t) (n:nat) (i:nat{i <= pow2 n}) =
+let rpmt (#hsz:pos) (#f:hash_fun_t) (n:nat) (i:nat{i <= pow2 n}) =
   mt:merkle_tree #hsz n {
-    raw_tages #_ #f (S.slice mt 0 i) /\
-    pad_tages #_ #f (S.slice mt i (S.length mt)) }
+    raw_hashes #_ #f (S.slice mt 0 i) /\
+    pad_hashes #_ #f (S.slice mt i (S.length mt)) }
 
-val rpmt_raws: #hsz:pos -> #f:tag_fun_t #hsz -> #n:nat -> #i:nat{i <= pow2 n} -> mt:rpmt #hsz #f n i -> S.seq (tag #hsz)
-let rpmt_raws #hsz #f #n #i mt = raw_tages_raws #_ #f (S.slice mt 0 i)
+val rpmt_raws: #hsz:pos -> #f:hash_fun_t #hsz -> #n:nat -> #i:nat{i <= pow2 n} -> mt:rpmt #hsz #f n i -> S.seq (hash #hsz)
+let rpmt_raws #hsz #f #n #i mt = raw_hashes_raws #_ #f (S.slice mt 0 i)
 
-val rpmt_i_0: #hsz:pos -> #f:tag_fun_t #hsz -> #n:nat -> mt:rpmt #hsz #f n 0 ->
+val rpmt_i_0: #hsz:pos -> #f:hash_fun_t #hsz -> #n:nat -> mt:rpmt #hsz #f n 0 ->
   Lemma (S.equal mt (S.create (pow2 n) (HPad #hsz)))
 let rpmt_i_0 #hsz #f #n mt = ()
 
-val rpmt_left: #hsz:pos -> #f:tag_fun_t #hsz -> #n:pos -> #i:nat{i <= pow2 n} -> rpmt #hsz #f n i ->
+val rpmt_left: #hsz:pos -> #f:hash_fun_t #hsz -> #n:pos -> #i:nat{i <= pow2 n} -> rpmt #hsz #f n i ->
   rpmt #hsz #f (n-1) (if i <= pow2 (n-1) then i else pow2 (n-1))
 let rpmt_left #hsz #f #n #i mt =
   if i <= pow2 (n-1)
-  then pad_tages_slice #_ #f (S.slice mt i (S.length mt)) 0 (pow2 (n-1) - i)
-  else raw_tages_slice #_ #f (S.slice mt 0 i) 0 (pow2 (n-1));
+  then pad_hashes_slice #_ #f (S.slice mt i (S.length mt)) 0 (pow2 (n-1) - i)
+  else raw_hashes_slice #_ #f (S.slice mt 0 i) 0 (pow2 (n-1));
   mt_left mt
 
 #push-options "--z3rlimit 40"
 
-val rpmt_right: #hsz:pos -> #f:tag_fun_t #hsz -> #n:pos -> #i:nat{i <= pow2 n} -> rpmt #hsz #f n i ->
+val rpmt_right: #hsz:pos -> #f:hash_fun_t #hsz -> #n:pos -> #i:nat{i <= pow2 n} -> rpmt #hsz #f n i ->
   rpmt #_ #f (n-1) (if i <= pow2 (n-1) then 0 else i - pow2 (n-1))
 let rpmt_right #hsz #f #n #i mt =
   if i <= pow2 (n-1)
-  then pad_tages_slice #_ #f (S.slice mt i (S.length mt)) (pow2 (n-1) - i) (pow2 n - i)
-  else raw_tages_slice #_ #f (S.slice mt 0 i) (pow2 (n-1)) i;
+  then pad_hashes_slice #_ #f (S.slice mt i (S.length mt)) (pow2 (n-1) - i) (pow2 n - i)
+  else raw_hashes_slice #_ #f (S.slice mt 0 i) (pow2 (n-1)) i;
   mt_right mt
 
 /// Two right-padded Merkle trees collide when
-/// 1) they have the same height (`n`) and number of raw tages (`i`),
+/// 1) they have the same height (`n`) and number of raw hashes (`i`),
 /// 2) their contents differ, and
 /// 3) their roots are same.
 
-// fournet: we may want to work towards removing 1) using a tag prefix
+// fournet: we may want to work towards removing 1) using a hash prefix
 noeq
-type mt_collide (#hsz:pos) (#f:tag_fun_t #hsz) (n:nat) (i:nat{i <= pow2 n}) = | Collision:
+type mt_collide (#hsz:pos) (#f:hash_fun_t #hsz) (n:nat) (i:nat{i <= pow2 n}) = | Collision:
   mt1:rpmt #_ #f n i -> mt2:rpmt #_ #f n i {
     mt1 =!= mt2 /\
     mt_get_root #_ #f #_ mt1 == mt_get_root #_ #f #_ mt2 } -> mt_collide #_ #f n i
 
 noeq
-type tag2_raw_collide = | Collision2:
-  #hsz:pos -> #f:tag_fun_t #hsz ->
-  lh1:tag -> rh1:tag ->
-  lh2:tag -> rh2:tag {
+type hash2_raw_collide = | Collision2:
+  #hsz:pos -> #f:hash_fun_t #hsz ->
+  lh1:hash -> rh1:hash ->
+  lh2:hash -> rh2:hash {
     (lh1 =!= lh2 \/ rh1 =!= rh2) /\
-    f lh1 rh1 == f lh2 rh2 } -> tag2_raw_collide
+    f lh1 rh1 == f lh2 rh2 } -> hash2_raw_collide
 
 /// Auxiliary lemmas for the proof
 
-val rpmt_pad_tages_0:
-  #hsz:pos -> #f:tag_fun_t #hsz ->
+val rpmt_pad_hashes_0:
+  #hsz:pos -> #f:hash_fun_t #hsz ->
   #n:nat -> #i:nat{i <= pow2 n} -> mt:rpmt #_ #f n i ->
-  Lemma (i = 0 <==> pad_tages #_ #f mt )
-let rpmt_pad_tages_0 #_ #_ #n #i mt = ()
+  Lemma (i = 0 <==> pad_hashes #_ #f mt )
+let rpmt_pad_hashes_0 #_ #_ #n #i mt = ()
 
-val rpmt_pad_tages_index_0:
-  #hsz:pos -> #f:tag_fun_t #hsz ->
+val rpmt_pad_hashes_index_0:
+  #hsz:pos -> #f:hash_fun_t #hsz ->
   #n:nat -> #i:nat{i <= pow2 n} ->
   mt:rpmt #_ #f n i ->
-  Lemma (pad_tages #_ #f mt <==> HPad? mt.[0])
-let rpmt_pad_tages_index_0 #_ #_ #n #i mt = ()
+  Lemma (pad_hashes #_ #f mt <==> HPad? mt.[0])
+let rpmt_pad_hashes_index_0 #_ #_ #n #i mt = ()
 
 val mt_get_root_pad_index_0:
-  #hsz:pos -> #f:tag_fun_t #hsz ->
+  #hsz:pos -> #f:hash_fun_t #hsz ->
   #n:nat -> mt:merkle_tree #hsz n ->
   Lemma (HPad? mt.[0] <==> HPad? (mt_get_root #_ #f mt))
 let rec mt_get_root_pad_index_0 #hsz #f #n (mt:merkle_tree #hsz n) =
@@ -456,35 +456,35 @@ let rec mt_get_root_pad_index_0 #hsz #f #n (mt:merkle_tree #hsz n) =
 
 #pop-options
 
-val rpmt_get_root_pad_tages:
-  #hsz:pos -> #f:tag_fun_t #hsz ->
+val rpmt_get_root_pad_hashes:
+  #hsz:pos -> #f:hash_fun_t #hsz ->
   #n:nat -> #i:nat{i <= pow2 n} -> mt:rpmt #_ #f n i ->
-  Lemma (pad_tages #_ #f mt <==> HPad? (mt_get_root #_ #f mt))
-let rpmt_get_root_pad_tages #_ #f #n #i mt =
-  rpmt_pad_tages_index_0 #_ #f mt;
+  Lemma (pad_hashes #_ #f mt <==> HPad? (mt_get_root #_ #f mt))
+let rpmt_get_root_pad_hashes #_ #f #n #i mt =
+  rpmt_pad_hashes_index_0 #_ #f mt;
   mt_get_root_pad_index_0 #_ #f mt
 
 val rpmt_get_root_pad:
-  #hsz:pos -> #f:tag_fun_t #hsz ->
+  #hsz:pos -> #f:hash_fun_t #hsz ->
   #n:nat -> #i:nat{i <= pow2 n} -> mt:rpmt #_ #f n i ->
   Lemma (i = 0 <==> HPad? (mt_get_root #_ #f mt))
 let rpmt_get_root_pad #_ #f #n #i mt =
-  rpmt_get_root_pad_tages #_ #f mt;
-  rpmt_pad_tages_0 #_ #f mt
+  rpmt_get_root_pad_hashes #_ #f mt;
+  rpmt_pad_hashes_0 #_ #f mt
 
 val rpmt_get_root_raw:
-  #hsz:pos -> #f:tag_fun_t #hsz ->
+  #hsz:pos -> #f:hash_fun_t #hsz ->
   #n:nat -> #i:nat{i <= pow2 n} -> mt:rpmt #_ #f n i ->
   Lemma (i > 0 <==> HRaw? (mt_get_root #_ #f mt))
 let rpmt_get_root_raw #hsz #f #n #i mt =
-  allow_inversion (padded_tag #hsz);
+  allow_inversion (padded_hash #hsz);
   rpmt_get_root_pad #_ #f mt
 
 #push-options "--z3rlimit 100"
 
 val extract: 
-  #hsz:pos -> #f:tag_fun_t #hsz ->
-  #n:nat -> #i:nat{i <= pow2 n} -> mt_collide #_ #f n i -> GTot tag2_raw_collide
+  #hsz:pos -> #f:hash_fun_t #hsz ->
+  #n:nat -> #i:nat{i <= pow2 n} -> mt_collide #_ #f n i -> GTot hash2_raw_collide
 let rec extract #hsz #f #n #i (Collision t1 t2) =
   assert(n = 0 ==> S.equal t1 t2); // excludes n = 0
   mt_left_right t1; mt_left_right t2;
