secure_api/merkle_tree/MerkleTree.New.Low.Datastructures.fst
@@ -1,0 +1,317 @@
+module MerkleTree.New.Low.Datastructures
+
+open FStar.All
+open FStar.Integers
+open FStar.Mul
+
+open LowStar.Buffer
+open LowStar.BufferOps
+open LowStar.Vector
+open LowStar.Regional
+open LowStar.RVector
+open LowStar.Regional.Instances
+
+module HS = FStar.HyperStack
+module HST = FStar.HyperStack.ST
+module MHS = FStar.Monotonic.HyperStack
+module HH = FStar.Monotonic.HyperHeap
+
+module B = LowStar.Buffer
+module CB = LowStar.ConstBuffer
+module V = LowStar.Vector
+module RV = LowStar.RVector
+module RVI = LowStar.Regional.Instances
+
+module S = FStar.Seq
+
+module EHS = EverCrypt.Hash
+module U32 = FStar.UInt32
+module MTH = MerkleTree.New.High
+
+open EverCrypt.Helpers
+open Lib.IntTypes
+
+open MerkleTree.New.Low.Hashes
+
+#set-options "--z3rlimit 10 --initial_fuel 0 --max_fuel 0 --initial_ifuel 0 --max_ifuel 0"
+
+// We cannot use `Low.RVector.Instances`, where we have some general
+// typeclass instances of `regional`, e.g., if `rg:regional a` then
+// `regional (rvector rg)`. In FStar we can use this, but KreMLin currently
+// cannot deal with this and gives a number of errors.
+// So we temporarily instantiate some `regional`s manually below, which is
+// extractable to C by KreMLin.
+
+/// Some instantiations of `regional` used in Merkle tree
+/// 1. `hash` is regional
+
+val hash_region_of: #hsz:hash_size_t -> v:hash #hsz -> GTot HH.rid
+let hash_region_of #_ v =
+  B.frameOf v
+
+noextract inline_for_extraction private
+val hash_dummy (#hsz:hash_size_t): hash #hsz
+let hash_dummy #hsz = B.null
+
+val hash_r_inv: #hsz:hash_size_t -> h:HS.mem -> v:hash #hsz -> GTot Type0
+let hash_r_inv #hsz h v =
+  B.live h v /\ B.freeable v /\
+  B.len v = hsz
+
+val hash_r_inv_reg:
+  #hsz:hash_size_t ->
+  h:HS.mem -> v:hash ->
+  Lemma (requires hash_r_inv h v)
+        (ensures MHS.live_region h (hash_region_of #hsz v))
+let hash_r_inv_reg #_ h v = ()
+
+private
+val hash_repr (#hsz:hash_size_t): Type0
+let hash_repr #hsz = MTH.hash #(U32.v hsz)
+
+val hash_r_repr: #hsz:hash_size_t -> h:HS.mem -> v:hash{hash_r_inv #hsz h v} -> GTot (hash_repr #hsz)
+let hash_r_repr #_ h v = B.as_seq h v
+
+val hash_r_sep:
+  #hsz:hash_size_t ->
+  v:hash #hsz -> p:loc -> h0:HS.mem -> h1:HS.mem ->
+  Lemma (requires
+      hash_r_inv h0 v /\
+      loc_disjoint
+        (loc_all_regions_from false
+          (hash_region_of v)) p /\
+      modifies p h0 h1)
+  (ensures
+     hash_r_inv h1 v /\
+     hash_r_repr h0 v == hash_r_repr h1 v)
+let hash_r_sep #_ v p h0 h1 =
+  assert (loc_includes (loc_all_regions_from false (hash_region_of v))
+                       (loc_buffer v));
+  B.modifies_buffer_elim v p h0 h1
+
+val hash_irepr: #hsz:hash_size_t -> Ghost.erased (hash_repr #hsz)
+let hash_irepr #hsz =
+  Ghost.hide (S.create (U32.v hsz) (u8 0))
+
+val hash_r_alloc_p: #hsz:hash_size_t -> v:hash #hsz -> GTot Type0
+let hash_r_alloc_p #_ v = True
+
+val hash_r_alloc:
+  #hsz:hash_size_t ->
+  r:HST.erid ->
+  HST.ST (hash #hsz)
+    (requires (fun h0 -> true))
+    (ensures (fun h0 v h1 ->
+      Set.subset (Map.domain (MHS.get_hmap h0))
+                 (Map.domain (MHS.get_hmap h1)) /\
+      modifies loc_none h0 h1 /\
+      hash_r_alloc_p v /\
+      hash_r_inv h1 v /\
+      hash_region_of v = r /\
+      hash_r_repr h1 v == Ghost.reveal hash_irepr /\
+      B.fresh_loc (B.loc_buffer v) h0 h1))
+let hash_r_alloc #hsz r =
+  B.malloc r (u8 0) hsz
+
+val hash_r_free:
+  #hsz:hash_size_t ->
+  v:hash #hsz ->
+  HST.ST unit
+    (requires fun h0 -> hash_r_inv h0 v)
+    (ensures  fun h0 _ h1 ->
+      modifies (loc_all_regions_from false (hash_region_of v)) h0 h1)
+let hash_r_free #_ v =
+  B.free v
+
+val hash_copy:
+  #hsz:hash_size_t ->
+  src:hash #hsz -> dst:hash #hsz ->
+  HST.ST unit
+    (requires fun h0 ->
+      hash_r_inv h0 src /\ hash_r_inv h0 dst /\
+      HH.disjoint (hash_region_of src) (hash_region_of dst))
+    (ensures fun h0 _ h1 ->
+      modifies (loc_all_regions_from false (hash_region_of dst)) h0 h1 /\
+      hash_r_inv h1 dst /\
+      hash_r_repr h1 dst == hash_r_repr h0 src)
+let hash_copy #hsz src dst =
+  B.blit src 0ul dst 0ul hsz
+
+noextract inline_for_extraction
+val hreg: #hsz:hash_size_t -> regional (hash #hsz)
+let hreg #hsz =
+  Rgl hash_region_of
+      B.loc_buffer
+      hash_dummy
+      hash_r_inv
+      hash_r_inv_reg
+      hash_repr
+      hash_r_repr
+      hash_r_sep
+      hash_irepr
+      hash_r_alloc_p
+      hash_r_alloc
+      hash_r_free
+
+val hcpy: #hsz:hash_size_t -> copyable (hash #hsz) hreg
+let hcpy #_ = Cpy hash_copy
+
+type hash_vec (#hsz:hash_size_t) = RV.rvector (hreg #hsz)
+
+/// 2. `rvector hash` is regional
+
+val hash_vec_region_of: #hsz:hash_size_t -> v:hash_vec #hsz -> GTot HH.rid
+let hash_vec_region_of #_ v = V.frameOf v
+
+private
+val hash_vec_dummy: #hsz:hash_size_t -> hash_vec #hsz
+let hash_vec_dummy #_ = V.alloc_empty hash
+
+val hash_vec_r_inv: #hsz:hash_size_t -> h:HS.mem -> v:hash_vec #hsz -> GTot Type0
+let hash_vec_r_inv #_ h v = RV.rv_inv h v
+
+val hash_vec_r_inv_reg:
+  #hsz:hash_size_t -> 
+  h:HS.mem -> v:hash_vec #hsz ->
+  Lemma (requires (hash_vec_r_inv h v))
+  (ensures (MHS.live_region h (hash_vec_region_of v)))
+let hash_vec_r_inv_reg #_ h v = ()
+
+private
+val hash_vec_repr: #hsz:hash_size_t -> Type0
+let hash_vec_repr #hsz = MTH.hashes #(U32.v hsz)
+
+val hash_vec_r_repr:
+  #hsz:hash_size_t -> 
+  h:HS.mem -> v:hash_vec #hsz {hash_vec_r_inv h v} -> GTot (hash_vec_repr #hsz)
+let hash_vec_r_repr #_ h v =
+  RV.as_seq h v
+
+val hash_vec_r_sep:
+  #hsz:hash_size_t -> 
+  v:hash_vec #hsz -> p:loc -> h0:HS.mem -> h1:HS.mem ->
+  Lemma (requires (hash_vec_r_inv h0 v /\
+      loc_disjoint
+        (loc_all_regions_from false (hash_vec_region_of v))
+        p /\
+      modifies p h0 h1))
+  (ensures (hash_vec_r_inv h1 v /\
+     hash_vec_r_repr h0 v == hash_vec_r_repr h1 v))
+let hash_vec_r_sep #_ v p h0 h1 =
+  RV.rv_inv_preserved v p h0 h1;
+  RV.as_seq_preserved v p h0 h1
+
+val hash_vec_irepr: #hsz:hash_size_t -> Ghost.erased (hash_vec_repr #hsz)
+let hash_vec_irepr #_ = Ghost.hide S.empty
+
+val hash_vec_r_alloc_p: #hsz:hash_size_t -> v:hash_vec #hsz -> GTot Type0
+let hash_vec_r_alloc_p #_ v = V.size_of v = 0ul
+
+#push-options "--initial_fuel 1 --max_fuel 1"
+val hash_vec_r_alloc:
+  #hsz:hash_size_t -> 
+  r:HST.erid ->
+  HST.ST (v:hash_vec #hsz)
+    (requires (fun h0 -> true))
+    (ensures (fun h0 v h1 ->
+      Set.subset (Map.domain (MHS.get_hmap h0))
+                 (Map.domain (MHS.get_hmap h1)) /\
+      modifies loc_none h0 h1 /\
+      hash_vec_r_alloc_p v /\
+      hash_vec_r_inv h1 v /\
+      hash_vec_region_of v = r /\
+      hash_vec_r_repr h1 v == Ghost.reveal hash_vec_irepr /\
+      B.fresh_loc (V.loc_vector v) h0 h1))
+let hash_vec_r_alloc #_ r =
+  let nrid = HST.new_region r in
+  let ia = Rgl?.dummy hreg in
+  V.alloc_reserve 1ul ia r
+#pop-options
+
+val hash_vec_r_free:
+  #hsz:hash_size_t -> 
+  v:hash_vec #hsz ->
+  HST.ST unit
+    (requires (fun h0 -> hash_vec_r_inv h0 v))
+    (ensures (fun h0 _ h1 ->
+      modifies (loc_all_regions_from false (hash_vec_region_of v)) h0 h1))
+let hash_vec_r_free #_ v =
+  RV.free v
+
+noextract inline_for_extraction
+val hvreg: #hsz:hash_size_t -> regional (hash_vec #hsz)
+let hvreg #_ =
+  Rgl hash_vec_region_of
+      V.loc_vector
+      hash_vec_dummy
+      hash_vec_r_inv
+      hash_vec_r_inv_reg
+      hash_vec_repr
+      hash_vec_r_repr
+      hash_vec_r_sep
+      hash_vec_irepr
+      hash_vec_r_alloc_p
+      hash_vec_r_alloc
+      hash_vec_r_free
+
+type hash_vv (#hsz:hash_size_t) = RV.rvector (hvreg #hsz)
+
+noextract
+val hvvreg: #hsz:hash_size_t -> regional (hash_vv #hsz)
+let hvvreg #_ = RVI.vector_regional hvreg
+
+val hash_vec_rv_inv_r_inv:
+  #hsz:hash_size_t ->
+  h:HS.mem -> hv:hash_vec #hsz -> i:uint32_t{i < V.size_of hv} ->
+  Lemma (requires RV.rv_inv h hv)
+        (ensures  Rgl?.r_inv hreg h (V.get h hv i))
+let hash_vec_rv_inv_r_inv #_ h hv i = ()
+
+val hash_vv_rv_inv_r_inv:
+  #hsz:hash_size_t ->
+  h:HS.mem -> hvv:hash_vv #hsz ->
+  i:uint32_t -> j:uint32_t ->
+  Lemma (requires RV.rv_inv h hvv /\
+                  i < V.size_of hvv /\
+                  j < V.size_of (V.get h hvv i))
+        (ensures Rgl?.r_inv hvreg h (V.get h hvv i) /\
+                 Rgl?.r_inv hreg h (V.get h (V.get h hvv i) j))
+let hash_vv_rv_inv_r_inv #_ h hvv i j = ()
+
+val hash_vv_rv_inv_disjoint:
+  #hsz:hash_size_t ->
+  h:HS.mem -> hvv:hash_vv #hsz ->
+  i:uint32_t -> j:uint32_t -> drid:HH.rid ->
+  Lemma (requires (RV.rv_inv h hvv /\
+                  i < V.size_of hvv /\
+                  j < V.size_of (V.get h hvv i) /\
+                  HH.disjoint (Rgl?.region_of hvvreg hvv) drid))
+        (ensures (HH.disjoint (Rgl?.region_of hreg (V.get h (V.get h hvv i) j)) drid))
+let hash_vv_rv_inv_disjoint #_ h hvv i j drid =
+  assert (HH.disjoint (Rgl?.region_of hvreg (V.get h hvv i)) drid);
+  assert (RV.rv_inv h (V.get h hvv i));
+  assert (HH.disjoint (Rgl?.region_of hreg (V.get h (V.get h hvv i) j)) drid)
+
+val hash_vv_rv_inv_includes:
+  #hsz:hash_size_t ->
+  h:HS.mem -> hvv:hash_vv #hsz ->
+  i:uint32_t -> j:uint32_t ->
+  Lemma (requires (RV.rv_inv h hvv /\
+                  i < V.size_of hvv /\
+                  j < V.size_of (V.get h hvv i)))
+        (ensures (HH.includes
+                   (Rgl?.region_of hvvreg hvv)
+                   (Rgl?.region_of hreg (V.get h (V.get h hvv i) j))))
+let hash_vv_rv_inv_includes #_ h hvv i j = ()
+
+val hash_vv_as_seq_get_index:
+  #hsz:hash_size_t ->
+  h:HS.mem -> hvv:hash_vv #hsz -> i:uint32_t -> j:uint32_t ->
+  Lemma (requires (RV.rv_inv h hvv /\
+                  i < V.size_of hvv /\
+                  j < V.size_of (V.get h hvv i)))
+        (ensures (Rgl?.r_repr hreg h (V.get h (V.get h hvv i) j) ==
+                 S.index (S.index (RV.as_seq h hvv) (U32.v i)) (U32.v j)))
+#push-options "--z3rlimit 20"
+let hash_vv_as_seq_get_index #_ h hvv i j = ()
+#pop-options
