secure_api/merkle_tree/MerkleTree.New.Low.Hashes.fst
@@ -1,0 +1,12 @@
+module MerkleTree.New.Low.Hashes
+
+module B = LowStar.Buffer
+module U32 = FStar.UInt32
+
+open FStar.Integers
+open EverCrypt.Helpers
+open Lib.IntTypes
+
+type hash_size_t = n:uint32_t{n > 0ul}
+type hash (#hsz:hash_size_t) = b:B.buffer uint8 { B.length b = (U32.v hsz) \/ B.g_is_null b }
+
