secure_api/merkle_tree/MerkleTree.New.Low.Hashfunctions.fst
@@ -1,0 +1,103 @@
+module MerkleTree.New.Low.Hashfunctions
+
+open EverCrypt.Helpers
+
+open FStar.All
+open FStar.Integers
+open FStar.Mul
+
+open LowStar.Buffer
+open LowStar.BufferOps
+open LowStar.Vector
+open LowStar.Regional
+open LowStar.RVector
+open LowStar.Regional.Instances
+
+module HS = FStar.HyperStack
+module HST = FStar.HyperStack.ST
+module MHS = FStar.Monotonic.HyperStack
+module HH = FStar.Monotonic.HyperHeap
+
+module B = LowStar.Buffer
+module CB = LowStar.ConstBuffer
+module V = LowStar.Vector
+module RV = LowStar.RVector
+module RVI = LowStar.Regional.Instances
+
+module S = FStar.Seq
+
+module U32 = FStar.UInt32
+module EHS = EverCrypt.Hash
+module MTH = MerkleTree.New.High
+module MTS = MerkleTree.Spec
+
+open Lib.IntTypes
+
+open MerkleTree.New.Low.Hashes
+open MerkleTree.New.Low.Datastructures
+
+#set-options "--z3rlimit 10 --initial_fuel 0 --max_fuel 0 --initial_ifuel 0 --max_ifuel 0"
+
+let init_hash (#hsz:hash_size_t) = hash_r_alloc #hsz
+let free_hash (#hsz:hash_size_t) = hash_r_free #hsz
+
+inline_for_extraction
+type hash_fun_t (#hsz:hash_size_t) (#hash_spec:MTS.hash_fun_t #(U32.v hsz)) = src1:hash #hsz -> src2:hash #hsz -> dst:hash #hsz -> HST.ST unit
+   (requires (fun h0 ->
+     Rgl?.r_inv hreg h0 src1 /\
+     Rgl?.r_inv hreg h0 src2 /\
+     Rgl?.r_inv hreg h0 dst))
+   (ensures (fun h0 _ h1 ->
+     // memory safety
+     modifies (B.loc_region_only false (B.frameOf dst)) h0 h1 /\
+     Rgl?.r_inv hreg h1 dst /\
+     // correctness
+     S.equal (Rgl?.r_repr hreg h1 dst)
+             (hash_spec (Rgl?.r_repr hreg h0 src1) (Rgl?.r_repr hreg h0 src2))
+     ))
+
+val sha256_compress: hash_fun_t #32ul #MTH.sha256_compress
+#push-options "--z3rlimit 40 --max_fuel 0"
+let sha256_compress src1 src2 dst =
+  let hash_size = 32ul in
+  let hash_alg = Spec.Hash.Definitions.SHA2_256 in
+  let hh0 = HST.get () in
+  HST.push_frame ();
+  // KreMLin can't extract `EHS.blockLen EHS.SHA256` (= 64ul)
+  let cb = B.alloca (u8 0) 64ul in
+  B.blit src1 0ul cb 0ul hash_size;
+  B.blit src2 0ul cb 32ul hash_size;
+
+  // ONLY WORKS BECAUSE hash_alg is inline_for_extraction and is known to be SHA2_256
+  let st = EHS.alloca hash_alg in
+  EHS.init #(Ghost.hide hash_alg) st;
+  let hh1 = HST.get () in
+  assert (S.equal (S.append
+                    (Rgl?.r_repr hreg hh0 src1)
+                    (Rgl?.r_repr hreg hh0 src2))
+                  (B.as_seq hh1 cb));
+
+  EHS.update #(Ghost.hide hash_alg) st cb;
+  let hh2 = HST.get () in
+  assert (EHS.repr st hh2 == Spec.Agile.Hash.update hash_alg (Spec.Agile.Hash.init hash_alg) (B.as_seq hh1 cb));
+  assert (S.equal (S.append S.empty (B.as_seq hh1 cb))
+                  (B.as_seq hh1 cb));
+
+  EHS.finish #(Ghost.hide hash_alg) st dst;
+  let hh3 = HST.get () in
+  assert (S.equal (B.as_seq hh3 dst)
+                  (Spec.Hash.PadFinish.finish hash_alg (EHS.repr st hh2)));
+  assert (S.equal (B.as_seq hh3 dst)
+                  (Spec.Hash.PadFinish.finish hash_alg (Spec.Agile.Hash.update hash_alg (Spec.Agile.Hash.init hash_alg) (B.as_seq hh1 cb))));
+  assert (S.equal (B.as_seq hh3 dst)
+                  (MTH.sha256_compress
+                    (Rgl?.r_repr hreg hh0 src1)
+                    (Rgl?.r_repr hreg hh0 src2)));
+  HST.pop_frame ();
+
+  let hh4 = HST.get () in
+  assert (S.equal (B.as_seq hh4 dst)
+                  (MTH.sha256_compress
+                    (Rgl?.r_repr hreg hh0 src1)
+                    (Rgl?.r_repr hreg hh0 src2)))
+#pop-options
